# Potenzgesetze
$$x^a \cdot x^b = x^{a+b}$$
$${x^a \over x^b} = x^{a-b}$$
$$(x^a)^b = x^{a \cdot b}$$
$$x^n \cdot y^n = (x \cdot y)^n$$
$${x^n \over y^n} = \left({x \over y}\right)^n$$
$$x^0 = 1$$
$$x^1=x$$
$$a^{-n} = {1 \over a^n}$$
$$\sqrt[m]{a^n} = a^{n \over m}$$
# Logarithmus
$b^c=a$ -> $\log_b(a)=c$ 
- $b$: Basis

$log_b(a) = 1$, wenn $a=b$
$\log_b(1)=0$, f√ºr alle $b$

# Limes
## Faktorregel:
$$\lim_{x \to \infty} c \cdot f(x) = c \cdot (\lim_{x \to \infty} f(x)) = c \cdot a$$
## Summenregel:
$$\lim_{x \to \infty} [f(x) + g(x)] = \lim_{x \to \infty} f(x) + \lim_{x \to \infty} g(x) = a + b$$
## Differenzregel:
$$\lim_{x \to \infty} [f(x) - g(x)] = \lim_{x \to \infty} f(x) - \lim_{x \to \infty} g(x) = a - b$$
## Produktregel:
$$\lim_{x \to \infty} [f(x) \cdot g(x)] = \lim_{x \to \infty} f(x) \cdot \lim_{x \to \infty} g(x) = a \cdot b$$
## Quotientenregel:
$$\lim_{x \to \infty} {f(x) \over g(x)} = {\lim_{x \to \infty} f(x) \over \lim_{x \to \infty} g(x)}= {a \over b}$$
## Logarithmusregel:
$$\lim_{x \to \infty} \log_{\alpha} f(x) = \log_{\alpha} (\lim_{x \to \infty} f(x)) = \log_{\alpha} a$$
## Potenzregel 1:
$$\lim_{x \to \infty} f(x)^{g(x)} = (\lim_{x\to \infty} f(x))^{\lim_{x \to \infty} g(x)} = a^b$$
**Voraussetzung**
$\lim_{x \to \infty} f(x) \ne 0$ und $\lim_{x \to \infty} g(x) \ne 0$ 
## Potenzregel 2:
$$\lim_{x \to \infty} (f(x))^p = (\lim_{x \to \infty} f(x))^p = a^p$$
## Potenzregel 3:
$$\lim_{x \to \infty} \sqrt[p]{f(x)} = \sqrt[p]{\lim_{x \to \infty} f(x)} = \sqrt[p]{a}$$
# Differenzieren
![[Differenzialrechnung#Potenzregel]]
![[Differenzialrechnung#Konstantenregel]]
![[Differenzialrechnung#Summenregel]]
![[Differenzialrechnung#Produktregel]]
![[Differenzialrechnung#Quotientenregel]]
![[Differenzialrechnung#Kettenregel]]
![[Differenzialrechnung#Ableitungen elementarer Funktionen]]
